src/Init/Data/String/Lemmas/Pattern/String/Basic.lean
@@ -20,17 +20,10 @@ namespace String.Slice.Pattern.Model
 namespace ForwardSliceSearcher
 
 instance {pat : Slice} : PatternModel pat where
-  /-
-  See the docstring of `PatternModel` for an explanation about why we disallow matching the
-  empty string.
+  Matches s := s = pat.copy
 
-  Requiring `s ≠ ""` is a trick that allows us to give a `PatternModel` instance
-  unconditionally, without forcing `pat.copy` to be non-empty (which would make it very awkward
-  to state theorems about the instance). It does not change anything about the fact that all lemmas
-  about this instance require `pat.isEmpty = false`.
-  -/
-  Matches s := s ≠ "" ∧ s = pat.copy
-  not_matches_empty := by simp
+theorem strictPatternModel {pat : Slice} (hpat : pat.isEmpty = false) : StrictPatternModel pat where
+  not_matches_empty := by simpa [PatternModel.Matches]
 
 instance {pat : Slice} : NoPrefixPatternModel pat :=
   .of_length_eq (by simp +contextual [PatternModel.Matches])
@@ -38,59 +31,52 @@ instance {pat : Slice} : NoPrefixPatternModel pat :=
 instance {pat : Slice} : NoSuffixPatternModel pat :=
   .of_length_eq (by simp +contextual [PatternModel.Matches])
 
-theorem isMatch_iff {pat s : Slice} {pos : s.Pos} (h : pat.isEmpty = false) :
+theorem isMatch_iff {pat s : Slice} {pos : s.Pos} :
     IsMatch pat pos ↔ (s.sliceTo pos).copy = pat.copy := by
-  simp only [Model.isMatch_iff, PatternModel.Matches, ne_eq, copy_eq_empty_iff,
-    Bool.not_eq_true, and_iff_right_iff_imp]
-  intro h'
-  rw [← isEmpty_copy (s := s.sliceTo pos), h', isEmpty_copy, h]
+  simp [Model.isMatch_iff, PatternModel.Matches]
 
-theorem isRevMatch_iff {pat s : Slice} {pos : s.Pos} (h : pat.isEmpty = false) :
+theorem isRevMatch_iff {pat s : Slice} {pos : s.Pos} :
     IsRevMatch pat pos ↔ (s.sliceFrom pos).copy = pat.copy := by
-  simp only [Model.isRevMatch_iff, PatternModel.Matches, ne_eq, copy_eq_empty_iff,
-    Bool.not_eq_true, and_iff_right_iff_imp]
-  intro h'
-  rw [← isEmpty_copy (s := s.sliceFrom pos), h', isEmpty_copy, h]
+  simp [Model.isRevMatch_iff, PatternModel.Matches]
 
-theorem isLongestMatch_iff {pat s : Slice} {pos : s.Pos} (h : pat.isEmpty = false) :
+theorem isLongestMatch_iff {pat s : Slice} {pos : s.Pos} :
     IsLongestMatch pat pos ↔ (s.sliceTo pos).copy = pat.copy := by
-  rw [isLongestMatch_iff_isMatch, isMatch_iff h]
+  rw [isLongestMatch_iff_isMatch, isMatch_iff]
 
-theorem isLongestRevMatch_iff {pat s : Slice} {pos : s.Pos} (h : pat.isEmpty = false) :
+theorem isLongestRevMatch_iff {pat s : Slice} {pos : s.Pos} :
     IsLongestRevMatch pat pos ↔ (s.sliceFrom pos).copy = pat.copy := by
-  rw [isLongestRevMatch_iff_isRevMatch, isRevMatch_iff h]
+  rw [isLongestRevMatch_iff_isRevMatch, isRevMatch_iff]
 
-theorem isLongestMatchAt_iff {pat s : Slice} {pos₁ pos₂ : s.Pos} (h : pat.isEmpty = false) :
+theorem isLongestMatchAt_iff {pat s : Slice} {pos₁ pos₂ : s.Pos} :
     IsLongestMatchAt pat pos₁ pos₂ ↔ ∃ h, (s.slice pos₁ pos₂ h).copy = pat.copy := by
-  simp [Model.isLongestMatchAt_iff, isLongestMatch_iff h]
+  simp [Model.isLongestMatchAt_iff, isLongestMatch_iff]
 
-theorem isLongestRevMatchAt_iff {pat s : Slice} {pos₁ pos₂ : s.Pos} (h : pat.isEmpty = false) :
+theorem isLongestRevMatchAt_iff {pat s : Slice} {pos₁ pos₂ : s.Pos} :
     IsLongestRevMatchAt pat pos₁ pos₂ ↔ ∃ h, (s.slice pos₁ pos₂ h).copy = pat.copy := by
-  simp [Model.isLongestRevMatchAt_iff, isLongestRevMatch_iff h]
+  simp [Model.isLongestRevMatchAt_iff, isLongestRevMatch_iff]
 
-theorem isLongestMatchAt_iff_splits {pat s : Slice} {pos₁ pos₂ : s.Pos} (h : pat.isEmpty = false) :
+theorem isLongestMatchAt_iff_splits {pat s : Slice} {pos₁ pos₂ : s.Pos} :
     IsLongestMatchAt pat pos₁ pos₂ ↔ ∃ t₁ t₂, pos₁.Splits t₁ (pat.copy ++ t₂) ∧
       pos₂.Splits (t₁ ++ pat.copy) t₂ := by
-  simp only [isLongestMatchAt_iff h, copy_slice_eq_iff_splits]
+  simp only [isLongestMatchAt_iff, copy_slice_eq_iff_splits]
 
-theorem isLongestRevMatchAt_iff_splits {pat s : Slice} {pos₁ pos₂ : s.Pos}
-    (h : pat.isEmpty = false) :
+theorem isLongestRevMatchAt_iff_splits {pat s : Slice} {pos₁ pos₂ : s.Pos} :
     IsLongestRevMatchAt pat pos₁ pos₂ ↔ ∃ t₁ t₂, pos₁.Splits t₁ (pat.copy ++ t₂) ∧
       pos₂.Splits (t₁ ++ pat.copy) t₂ := by
-  simp only [isLongestRevMatchAt_iff h, copy_slice_eq_iff_splits]
+  simp only [isLongestRevMatchAt_iff, copy_slice_eq_iff_splits]
 
-theorem isLongestMatch_iff_splits {pat s : Slice} {pos : s.Pos} (h : pat.isEmpty = false) :
+theorem isLongestMatch_iff_splits {pat s : Slice} {pos : s.Pos} :
     IsLongestMatch pat pos ↔ ∃ t, pos.Splits pat.copy t := by
-  rw [isLongestMatch_iff h, copy_sliceTo_eq_iff_exists_splits]
+  rw [isLongestMatch_iff, copy_sliceTo_eq_iff_exists_splits]
 
-theorem isLongestRevMatch_iff_splits {pat s : Slice} {pos : s.Pos} (h : pat.isEmpty = false) :
+theorem isLongestRevMatch_iff_splits {pat s : Slice} {pos : s.Pos} :
     IsLongestRevMatch pat pos ↔ ∃ t, pos.Splits t pat.copy := by
-  rw [isLongestRevMatch_iff h, copy_sliceFrom_eq_iff_exists_splits]
+  rw [isLongestRevMatch_iff, copy_sliceFrom_eq_iff_exists_splits]
 
 theorem isLongestMatchAt_iff_extract {pat s : Slice} {pos₁ pos₂ : s.Pos} (h : pat.isEmpty = false) :
     IsLongestMatchAt pat pos₁ pos₂ ↔
       s.copy.toByteArray.extract pos₁.offset.byteIdx pos₂.offset.byteIdx = pat.copy.toByteArray := by
-  rw [isLongestMatchAt_iff h]
+  rw [isLongestMatchAt_iff]
   refine ⟨fun ⟨h, h'⟩ => ?_, fun h' => ?_⟩
   · simp [← h', toByteArray_copy_slice]
   · rw [← Slice.toByteArray_copy_ne_empty_iff, ← h', ne_eq, ByteArray.extract_eq_empty_iff] at h
@@ -102,7 +88,7 @@ theorem isLongestRevMatchAt_iff_extract {pat s : Slice} {pos₁ pos₂ : s.Pos}
     IsLongestRevMatchAt pat pos₁ pos₂ ↔
       s.copy.toByteArray.extract pos₁.offset.byteIdx pos₂.offset.byteIdx =
         pat.copy.toByteArray := by
-  rw [isLongestRevMatchAt_iff h]
+  rw [isLongestRevMatchAt_iff]
   refine ⟨fun ⟨h, h'⟩ => ?_, fun h' => ?_⟩
   · simp [← h', toByteArray_copy_slice]
   · rw [← Slice.toByteArray_copy_ne_empty_iff, ← h', ne_eq, ByteArray.extract_eq_empty_iff] at h
@@ -130,21 +116,21 @@ theorem offset_of_isLongestRevMatchAt {pat s : Slice} {pos₁ pos₂ : s.Pos}
   suffices pos₂.offset.byteIdx ≤ s.utf8ByteSize by omega
   simpa [Pos.le_iff, Pos.Raw.le_iff] using pos₂.le_endPos
 
-theorem matchesAt_iff_splits {pat s : Slice} {pos : s.Pos} (h : pat.isEmpty = false) :
+theorem matchesAt_iff_splits {pat s : Slice} {pos : s.Pos} :
     MatchesAt pat pos ↔ ∃ t₁ t₂, pos.Splits t₁ (pat.copy ++ t₂) := by
-  simp only [matchesAt_iff_exists_isLongestMatchAt, isLongestMatchAt_iff_splits h]
+  simp only [matchesAt_iff_exists_isLongestMatchAt, isLongestMatchAt_iff_splits]
   exact ⟨fun ⟨e, t₁, t₂, ht₁, ht₂⟩ => ⟨t₁, t₂, ht₁⟩,
     fun ⟨t₁, t₂, ht⟩ => ⟨ht.rotateRight, t₁, t₂, ht, ht.splits_rotateRight⟩⟩
 
-theorem revMatchesAt_iff_splits {pat s : Slice} {pos : s.Pos} (h : pat.isEmpty = false) :
+theorem revMatchesAt_iff_splits {pat s : Slice} {pos : s.Pos} :
     RevMatchesAt pat pos ↔ ∃ t₁ t₂, pos.Splits (t₁ ++ pat.copy) t₂ := by
-  simp only [revMatchesAt_iff_exists_isLongestRevMatchAt, isLongestRevMatchAt_iff_splits h]
+  simp only [revMatchesAt_iff_exists_isLongestRevMatchAt, isLongestRevMatchAt_iff_splits]
   exact ⟨fun ⟨e, t₁, t₂, ht₁, ht₂⟩ => ⟨t₁, t₂, ht₂⟩,
     fun ⟨t₁, t₂, ht⟩ => ⟨ht.rotateLeft, t₁, t₂, ht.splits_rotateLeft, ht⟩⟩
 
-theorem exists_matchesAt_iff_eq_append {pat s : Slice} (h : pat.isEmpty = false) :
+theorem exists_matchesAt_iff_eq_append {pat s : Slice} :
     (∃ (pos : s.Pos), MatchesAt pat pos) ↔ ∃ t₁ t₂, s.copy = t₁ ++ pat.copy ++ t₂ := by
-  simp only [matchesAt_iff_splits h]
+  simp only [matchesAt_iff_splits]
   constructor
   · rintro ⟨pos, t₁, t₂, hsplit⟩
     exact ⟨t₁, t₂, by rw [hsplit.eq_append, append_assoc]⟩
@@ -154,9 +140,9 @@ theorem exists_matchesAt_iff_eq_append {pat s : Slice} (h : pat.isEmpty = false)
         ⟨t₁, pat.copy ++ t₂, by rw [← append_assoc]; exact heq, rfl⟩
     exact ⟨s.pos _ hvalid, t₁, t₂, ⟨by rw [← append_assoc]; exact heq, by simp⟩⟩
 
-theorem exists_revMatchesAt_iff_eq_append {pat s : Slice} (h : pat.isEmpty = false) :
+theorem exists_revMatchesAt_iff_eq_append {pat s : Slice} :
     (∃ (pos : s.Pos), RevMatchesAt pat pos) ↔ ∃ t₁ t₂, s.copy = t₁ ++ pat.copy ++ t₂ := by
-  simp only [revMatchesAt_iff_splits h]
+  simp only [revMatchesAt_iff_splits]
   constructor
   · rintro ⟨pos, t₁, t₂, hsplit⟩
     exact ⟨t₁, t₂, by rw [hsplit.eq_append, append_assoc]⟩
@@ -233,8 +219,10 @@ end ForwardSliceSearcher
 namespace ForwardStringSearcher
 
 instance {pat : String} : PatternModel pat where
-  Matches s := s ≠ "" ∧ s = pat
-  not_matches_empty := by simp
+  Matches s := s = pat
+
+theorem strictPatternModel {pat : String} (h : pat ≠ "") : StrictPatternModel pat where
+  not_matches_empty := by simpa [PatternModel.Matches]
 
 instance {pat : String} : NoPrefixPatternModel pat :=
   .of_length_eq (by simp +contextual [PatternModel.Matches])
@@ -282,61 +270,55 @@ theorem revMatchesAt_iff_toSlice {pat : String} {s : Slice} {pos : s.Pos} :
   simp [revMatchesAt_iff_exists_isLongestRevMatchAt,
     isLongestRevMatchAt_iff_isLongestRevMatchAt_toSlice]
 
-private theorem toSlice_isEmpty (h : pat ≠ "") : pat.toSlice.isEmpty = false := by
-  rwa [isEmpty_toSlice, isEmpty_eq_false_iff]
-
-theorem isMatch_iff {pat : String} {s : Slice} {pos : s.Pos} (h : pat ≠ "") :
+theorem isMatch_iff {pat : String} {s : Slice} {pos : s.Pos} :
     IsMatch pat pos ↔ (s.sliceTo pos).copy = pat := by
-  rw [isMatch_iff_slice, ForwardSliceSearcher.isMatch_iff (toSlice_isEmpty h)]
+  rw [isMatch_iff_slice, ForwardSliceSearcher.isMatch_iff]
   simp
 
-theorem isRevMatch_iff {pat : String} {s : Slice} {pos : s.Pos} (h : pat ≠ "") :
+theorem isRevMatch_iff {pat : String} {s : Slice} {pos : s.Pos} :
     IsRevMatch pat pos ↔ (s.sliceFrom pos).copy = pat := by
-  rw [isRevMatch_iff_slice, ForwardSliceSearcher.isRevMatch_iff (toSlice_isEmpty h)]
+  rw [isRevMatch_iff_slice, ForwardSliceSearcher.isRevMatch_iff]
   simp
 
-theorem isLongestMatch_iff {pat : String} {s : Slice} {pos : s.Pos} (h : pat ≠ "") :
+theorem isLongestMatch_iff {pat : String} {s : Slice} {pos : s.Pos} :
     IsLongestMatch pat pos ↔ (s.sliceTo pos).copy = pat := by
-  rw [isLongestMatch_iff_isMatch, isMatch_iff h]
+  rw [isLongestMatch_iff_isMatch, isMatch_iff]
 
-theorem isLongestRevMatch_iff {pat : String} {s : Slice} {pos : s.Pos} (h : pat ≠ "") :
+theorem isLongestRevMatch_iff {pat : String} {s : Slice} {pos : s.Pos} :
     IsLongestRevMatch pat pos ↔ (s.sliceFrom pos).copy = pat := by
-  rw [isLongestRevMatch_iff_isRevMatch, isRevMatch_iff h]
+  rw [isLongestRevMatch_iff_isRevMatch, isRevMatch_iff]
 
-theorem isLongestMatchAt_iff {pat : String} {s : Slice} {pos₁ pos₂ : s.Pos} (h : pat ≠ "") :
+theorem isLongestMatchAt_iff {pat : String} {s : Slice} {pos₁ pos₂ : s.Pos} :
     IsLongestMatchAt pat pos₁ pos₂ ↔ ∃ h, (s.slice pos₁ pos₂ h).copy = pat := by
   rw [isLongestMatchAt_iff_isLongestMatchAt_toSlice,
-    ForwardSliceSearcher.isLongestMatchAt_iff (toSlice_isEmpty h)]
+    ForwardSliceSearcher.isLongestMatchAt_iff]
   simp
 
-theorem isLongestRevMatchAt_iff {pat : String} {s : Slice} {pos₁ pos₂ : s.Pos} (h : pat ≠ "") :
+theorem isLongestRevMatchAt_iff {pat : String} {s : Slice} {pos₁ pos₂ : s.Pos} :
     IsLongestRevMatchAt pat pos₁ pos₂ ↔ ∃ h, (s.slice pos₁ pos₂ h).copy = pat := by
   rw [isLongestRevMatchAt_iff_isLongestRevMatchAt_toSlice,
-    ForwardSliceSearcher.isLongestRevMatchAt_iff (toSlice_isEmpty h)]
+    ForwardSliceSearcher.isLongestRevMatchAt_iff]
   simp
 
-theorem isLongestMatchAt_iff_splits {pat : String} {s : Slice} {pos₁ pos₂ : s.Pos}
-    (h : pat ≠ "") :
+theorem isLongestMatchAt_iff_splits {pat : String} {s : Slice} {pos₁ pos₂ : s.Pos} :
     IsLongestMatchAt pat pos₁ pos₂ ↔
       ∃ t₁ t₂, pos₁.Splits t₁ (pat ++ t₂) ∧ pos₂.Splits (t₁ ++ pat) t₂ := by
   rw [isLongestMatchAt_iff_isLongestMatchAt_toSlice,
-    ForwardSliceSearcher.isLongestMatchAt_iff_splits (toSlice_isEmpty h)]
+    ForwardSliceSearcher.isLongestMatchAt_iff_splits]
   simp
 
-theorem isLongestRevMatchAt_iff_splits {pat : String} {s : Slice} {pos₁ pos₂ : s.Pos}
-    (h : pat ≠ "") :
+theorem isLongestRevMatchAt_iff_splits {pat : String} {s : Slice} {pos₁ pos₂ : s.Pos} :
     IsLongestRevMatchAt pat pos₁ pos₂ ↔
       ∃ t₁ t₂, pos₁.Splits t₁ (pat ++ t₂) ∧ pos₂.Splits (t₁ ++ pat) t₂ := by
   rw [isLongestRevMatchAt_iff_isLongestRevMatchAt_toSlice,
-    ForwardSliceSearcher.isLongestRevMatchAt_iff_splits (toSlice_isEmpty h)]
+    ForwardSliceSearcher.isLongestRevMatchAt_iff_splits]
   simp
 
-theorem isLongestMatchAt_iff_extract {pat : String} {s : Slice} {pos₁ pos₂ : s.Pos}
-    (h : pat ≠ "") :
+theorem isLongestMatchAt_iff_extract {pat : String} {s : Slice} {pos₁ pos₂ : s.Pos} (h : pat ≠ "") :
     IsLongestMatchAt pat pos₁ pos₂ ↔
       s.copy.toByteArray.extract pos₁.offset.byteIdx pos₂.offset.byteIdx = pat.toByteArray := by
   rw [isLongestMatchAt_iff_isLongestMatchAt_toSlice,
-    ForwardSliceSearcher.isLongestMatchAt_iff_extract (toSlice_isEmpty h)]
+    ForwardSliceSearcher.isLongestMatchAt_iff_extract (by simpa)]
   simp
 
 theorem isLongestRevMatchAt_iff_extract {pat : String} {s : Slice} {pos₁ pos₂ : s.Pos}
@@ -344,38 +326,38 @@ theorem isLongestRevMatchAt_iff_extract {pat : String} {s : Slice} {pos₁ pos�
     IsLongestRevMatchAt pat pos₁ pos₂ ↔
       s.copy.toByteArray.extract pos₁.offset.byteIdx pos₂.offset.byteIdx = pat.toByteArray := by
   rw [isLongestRevMatchAt_iff_isLongestRevMatchAt_toSlice,
-    ForwardSliceSearcher.isLongestRevMatchAt_iff_extract (toSlice_isEmpty h)]
+    ForwardSliceSearcher.isLongestRevMatchAt_iff_extract (by simpa)]
   simp
 
 theorem offset_of_isLongestMatchAt {pat : String} {s : Slice} {pos₁ pos₂ : s.Pos}
     (h : pat ≠ "") (h' : IsLongestMatchAt pat pos₁ pos₂) :
     pos₂.offset = pos₁.offset.increaseBy pat.utf8ByteSize := by
   rw [show pat.utf8ByteSize = pat.toSlice.utf8ByteSize from utf8ByteSize_toSlice.symm]
-  exact ForwardSliceSearcher.offset_of_isLongestMatchAt (toSlice_isEmpty h)
+  exact ForwardSliceSearcher.offset_of_isLongestMatchAt (by simpa)
     (isLongestMatchAt_iff_isLongestMatchAt_toSlice.1 h')
 
 theorem offset_of_isLongestRevMatchAt {pat : String} {s : Slice} {pos₁ pos₂ : s.Pos}
     (h : pat ≠ "") (h' : IsLongestRevMatchAt pat pos₁ pos₂) :
     pos₂.offset = pos₁.offset.increaseBy pat.utf8ByteSize := by
   rw [show pat.utf8ByteSize = pat.toSlice.utf8ByteSize from utf8ByteSize_toSlice.symm]
-  exact ForwardSliceSearcher.offset_of_isLongestRevMatchAt (toSlice_isEmpty h)
+  exact ForwardSliceSearcher.offset_of_isLongestRevMatchAt (by simpa)
     (isLongestRevMatchAt_iff_isLongestRevMatchAt_toSlice.1 h')
 
-theorem matchesAt_iff_splits {pat : String} {s : Slice} {pos : s.Pos} (h : pat ≠ "") :
+theorem matchesAt_iff_splits {pat : String} {s : Slice} {pos : s.Pos} :
     MatchesAt pat pos ↔ ∃ t₁ t₂, pos.Splits t₁ (pat ++ t₂) := by
   rw [matchesAt_iff_toSlice,
-    ForwardSliceSearcher.matchesAt_iff_splits (toSlice_isEmpty h)]
+    ForwardSliceSearcher.matchesAt_iff_splits]
   simp
 
-theorem revMatchesAt_iff_splits {pat : String} {s : Slice} {pos : s.Pos} (h : pat ≠ "") :
+theorem revMatchesAt_iff_splits {pat : String} {s : Slice} {pos : s.Pos} :
     RevMatchesAt pat pos ↔ ∃ t₁ t₂, pos.Splits (t₁ ++ pat) t₂ := by
   rw [revMatchesAt_iff_toSlice,
-    ForwardSliceSearcher.revMatchesAt_iff_splits (toSlice_isEmpty h)]
+    ForwardSliceSearcher.revMatchesAt_iff_splits]
   simp
 
-theorem exists_matchesAt_iff_eq_append {pat : String} {s : Slice} (h : pat ≠ "") :
+theorem exists_matchesAt_iff_eq_append {pat : String} {s : Slice} :
     (∃ (pos : s.Pos), MatchesAt pat pos) ↔ ∃ t₁ t₂, s.copy = t₁ ++ pat ++ t₂ := by
-  simp only [matchesAt_iff_splits h]
+  simp only [matchesAt_iff_splits]
   constructor
   · rintro ⟨pos, t₁, t₂, hsplit⟩
     exact ⟨t₁, t₂, by rw [hsplit.eq_append, append_assoc]⟩
@@ -385,12 +367,12 @@ theorem exists_matchesAt_iff_eq_append {pat : String} {s : Slice} (h : pat ≠ "
         ⟨t₁, pat ++ t₂, by rw [← append_assoc]; exact heq, rfl⟩
     exact ⟨s.pos _ hvalid, t₁, t₂, ⟨by rw [← append_assoc]; exact heq, by simp⟩⟩
 
-theorem exists_revMatchesAt_iff_eq_append {pat : String} {s : Slice} (h : pat ≠ "") :
+theorem exists_revMatchesAt_iff_eq_append {pat : String} {s : Slice} :
     (∃ (pos : s.Pos), RevMatchesAt pat pos) ↔ ∃ t₁ t₂, s.copy = t₁ ++ pat ++ t₂ := by
   rw [show (∃ (pos : s.Pos), RevMatchesAt (ρ := String) pat pos) ↔
       (∃ (pos : s.Pos), RevMatchesAt (ρ := Slice) pat.toSlice pos) from by
     simp [revMatchesAt_iff_toSlice],
-    ForwardSliceSearcher.exists_revMatchesAt_iff_eq_append (toSlice_isEmpty h)]
+    ForwardSliceSearcher.exists_revMatchesAt_iff_eq_append]
   simp
 
 theorem matchesAt_iff_isLongestMatchAt {pat : String} {s : Slice} {pos : s.Pos}
@@ -398,7 +380,7 @@ theorem matchesAt_iff_isLongestMatchAt {pat : String} {s : Slice} {pos : s.Pos}
     MatchesAt pat pos ↔ ∃ (h : (pos.offset.increaseBy pat.utf8ByteSize).IsValidForSlice s),
       IsLongestMatchAt pat pos (s.pos _ h) := by
   have key := ForwardSliceSearcher.matchesAt_iff_isLongestMatchAt (pat := pat.toSlice)
-    (toSlice_isEmpty h) (pos := pos)
+    (by simpa) (pos := pos)
   simp only [utf8ByteSize_toSlice, ← isLongestMatchAt_iff_isLongestMatchAt_toSlice] at key
   rwa [matchesAt_iff_toSlice]
 
@@ -408,7 +390,7 @@ theorem revMatchesAt_iff_isLongestRevMatchAt {pat : String} {s : Slice} {pos : s
       ∃ (h : (pos.offset.decreaseBy pat.utf8ByteSize).IsValidForSlice s),
         IsLongestRevMatchAt pat (s.pos _ h) pos := by
   have key := ForwardSliceSearcher.revMatchesAt_iff_isLongestRevMatchAt (pat := pat.toSlice)
-    (toSlice_isEmpty h) (pos := pos)
+    (by simpa) (pos := pos)
   simp only [utf8ByteSize_toSlice, ← isLongestRevMatchAt_iff_isLongestRevMatchAt_toSlice] at key
   rwa [revMatchesAt_iff_toSlice]
 
@@ -418,14 +400,14 @@ theorem matchesAt_iff_getElem {pat : String} {s : Slice} {pos : s.Pos} (h : pat 
         ∀ (j), (hj : j < pat.toByteArray.size) →
           pat.toByteArray[j] = s.copy.toByteArray[pos.offset.byteIdx + j] := by
   have key := ForwardSliceSearcher.matchesAt_iff_getElem (pat := pat.toSlice)
-    (toSlice_isEmpty h) (pos := pos)
+    (by simpa) (pos := pos)
   simp only [copy_toSlice] at key
   rwa [matchesAt_iff_toSlice]
 
 theorem le_of_matchesAt {pat : String} {s : Slice} {pos : s.Pos} (h : pat ≠ "")
     (h' : MatchesAt pat pos) : pos.offset.increaseBy pat.utf8ByteSize ≤ s.rawEndPos := by
   rw [show pat.utf8ByteSize = pat.toSlice.utf8ByteSize from utf8ByteSize_toSlice.symm]
-  exact ForwardSliceSearcher.le_of_matchesAt (toSlice_isEmpty h)
+  exact ForwardSliceSearcher.le_of_matchesAt (by simpa)
     (matchesAt_iff_toSlice.1 h')
 
 theorem matchesAt_iff_matchesAt_toSlice {pat : String} {s : Slice}
