src/Init/Data/String/Lemmas/Pattern/TakeDrop/Basic.lean
@@ -11,6 +11,8 @@ public import Init.Data.String.TakeDrop
 public import Init.Data.String.Lemmas.Pattern.Basic
 import all Init.Data.String.Slice
 import all Init.Data.String.TakeDrop
+import Init.Data.String.Lemmas.Intercalate
+import Init.Data.String.Lemmas.Basic
 
 public section
 
@@ -72,6 +74,164 @@ theorem Pattern.Model.eq_append_of_dropPrefix?_eq_some {ρ : Type} {pat : ρ} [P
   obtain ⟨pos, h₁, h₂⟩ := h
   exact ⟨(s.sliceTo pos).copy, h₁.isMatch.matches_copy, by simp [← h₂, ← copy_eq_copy_sliceTo]⟩
 
+theorem Pos.skip?_eq_map_skipPrefix? {ρ : Type} {pat : ρ} [ForwardPattern pat] {s : Slice} {pos : s.Pos} :
+    pos.skip? pat = ((s.sliceFrom pos).skipPrefix? pat).map Pos.ofSliceFrom :=
+  (rfl)
+
+theorem Pattern.Model.Pos.skip?_eq_some_iff {ρ : Type} {pat : ρ} [PatternModel pat] [ForwardPattern pat]
+    [LawfulForwardPatternModel pat] {s : Slice} {pos res : s.Pos} :
+    pos.skip? pat = some res ↔ IsLongestMatchAt pat pos res := by
+  simp only [Pos.skip?_eq_map_skipPrefix?, Option.map_eq_some_iff, skipPrefix?_eq_some_iff,
+    isLongestMatchAt_iff]
+  refine ⟨?_, ?_⟩
+  · rintro ⟨p, ⟨h, rfl⟩⟩
+    simpa
+  · rintro ⟨h, h'⟩
+    exact ⟨Pos.sliceFrom _ _ h, by simpa⟩
+
+theorem Pattern.Model.Pos.skip?_eq_none_iff {ρ : Type} {pat : ρ} [PatternModel pat] [ForwardPattern pat]
+    [LawfulForwardPatternModel pat] {s : Slice} {pos : s.Pos} :
+    pos.skip? pat = none ↔ ¬ MatchesAt pat pos := by
+  simp [Pos.skip?_eq_map_skipPrefix?, startsWith_eq_false_iff, matchesAt_iff_matchesAt_ofSliceFrom]
+
+theorem Pattern.Model.Pos.skip?_eq_matchAt? {ρ : Type} {pat : ρ} [PatternModel pat] [ForwardPattern pat]
+    [LawfulForwardPatternModel pat] {s : Slice} {pos : s.Pos} :
+    pos.skip? pat = matchAt? pat pos :=
+  Option.ext (fun res => by simp [Pattern.Model.Pos.skip?_eq_some_iff])
+
+@[simp]
+theorem skip?_startPos {ρ : Type} {pat : ρ} [PatternModel pat] [ForwardPattern pat] [LawfulForwardPatternModel pat]
+    {s : Slice} : s.startPos.skip? pat = s.skipPrefix? pat :=
+  Option.ext (fun pos => by simp [Pattern.Model.skipPrefix?_eq_some_iff, Pattern.Model.Pos.skip?_eq_some_iff])
+
+theorem Pos.skip?_cast {ρ : Type} {pat : ρ} [PatternModel pat] [ForwardPattern pat] [LawfulForwardPatternModel pat]
+    {s t : Slice} (hst : s.copy = t.copy) {pos : s.Pos} :
+    (pos.cast hst).skip? pat = (pos.skip? pat).map (·.cast hst) := by
+  simp [Pattern.Model.Pos.skip?_eq_matchAt?, matchAt?_cast]
+
+theorem Pos.skip?_congr {ρ : Type} {pat : ρ} [PatternModel pat] [ForwardPattern pat] [LawfulForwardPatternModel pat]
+    {s t : Slice} (hst : s.copy = t.copy) {pos : s.Pos} :
+    pos.skip? pat = ((pos.cast hst).skip? pat).map (·.cast hst.symm) := by
+  simp only [skip?_cast, Option.map_map]
+  conv => lhs; rw [← Option.map_id_apply (x := pos.skip? pat)]
+  congr
+  ext; simp
+
+theorem skipPrefix?_congr {ρ : Type} {pat : ρ} [PatternModel pat] [ForwardPattern pat]
+    [LawfulForwardPatternModel pat] {s t : Slice} (hst : s.copy = t.copy) :
+    s.skipPrefix? pat = (t.skipPrefix? pat).map (·.cast hst.symm) := by
+  rw [← skip?_startPos, ← Pos.cast_startPos (hst := hst.symm), Pos.skip?_cast, skip?_startPos]
+
+theorem startsWith_congr {ρ : Type} {pat : ρ} [PatternModel pat] [ForwardPattern pat]
+    [LawfulForwardPatternModel pat] {s t : Slice} (hst : s.copy = t.copy) :
+    s.startsWith pat = t.startsWith pat := by
+  rw [← isSome_skipPrefix?, skipPrefix?_congr hst, Option.isSome_map, isSome_skipPrefix?]
+
+theorem dropPrefix?_congr {ρ : Type} {pat : ρ} [PatternModel pat] [ForwardPattern pat]
+    [LawfulForwardPatternModel pat] {s t : Slice} (hst : s.copy = t.copy) :
+    (s.dropPrefix? pat).map String.Slice.copy = (t.dropPrefix? pat).map String.Slice.copy := by
+  simp only [dropPrefix?_eq_map_skipPrefix?]
+  rw [skipPrefix?_congr hst]
+  simp only [Option.map_map]
+  congr 1
+  ext
+  simp
+
+theorem Pattern.Model.Pos.skipWhile_eq {ρ : Type} {pat : ρ} [PatternModel pat] [StrictPatternModel pat]
+    [ForwardPattern pat] [LawfulForwardPatternModel pat] {s : Slice} {pos : s.Pos} :
+    pos.skipWhile pat = (matchAt? pat pos).elim pos (·.skipWhile pat) := by
+  fun_induction Pos.skipWhile with
+  | case1 pos nextCurr h₁ h₂ ih =>
+    rw [Pattern.Model.Pos.skip?_eq_matchAt?] at h₁
+    simp [h₁]
+  | case2 pos nextCurr h₁ h₂ =>
+    rw [Pattern.Model.Pos.skip?_eq_some_iff] at h₁
+    exact (h₂ h₁.lt).elim
+  | case3 p h =>
+    rw [Pattern.Model.Pos.skip?_eq_matchAt?] at h
+    simp [h]
+
+theorem Pos.skipWhile_cast {ρ : Type} {pat : ρ} [PatternModel pat] [ForwardPattern pat]
+    [LawfulForwardPatternModel pat] {s t : Slice} (hst : s.copy = t.copy) {pos : s.Pos} :
+    (pos.cast hst).skipWhile pat = (pos.skipWhile pat).cast hst := by
+  fun_induction Pos.skipWhile with
+  | case1 pos nextCurr h₁ h₂ ih =>
+    rw [← ih, skipWhile]
+    simp [skip?_cast, h₁, h₂]
+  | case2 pos nextCurr h₁ h₂ =>
+    rw [skipWhile]
+    simp [skip?_cast, h₁, h₂]
+  | case3 p h =>
+    rw [skipWhile]
+    simp [skip?_cast, h]
+
+theorem Pos.skipWhile_congr {ρ : Type} {pat : ρ} [PatternModel pat] [ForwardPattern pat]
+    [LawfulForwardPatternModel pat] {s t : Slice} (hst : s.copy = t.copy) {pos : s.Pos} :
+    pos.skipWhile pat = ((pos.cast hst).skipWhile pat).cast hst.symm := by
+  simp [Pos.skipWhile_cast]
+
+theorem Pattern.Model.Pos.exists_eq_of_skipWhile_eq {ρ : Type} {pat : ρ} [PatternModel pat] [StrictPatternModel pat]
+    [ForwardPattern pat]
+    [LawfulForwardPatternModel pat] {s : Slice} {pos res : s.Pos} (h : pos.skipWhile pat = res) :
+    ∃ (l : List String),
+      (∀ t ∈ l, PatternModel.Matches pat t) ∧ ¬MatchesAt pat res ∧ (s.sliceFrom pos).copy = String.join l ++ (s.sliceFrom res).copy := by
+  subst h
+  induction pos using WellFounded.induction Pos.wellFounded_gt with | h pos ih
+  match hpos : matchAt? pat pos with
+  | some nextCurr =>
+    rw [skipWhile_eq]
+    simp only [hpos, Option.elim_some]
+    rw [matchAt?_eq_some_iff] at hpos
+    obtain ⟨l, hl₁, hl₂, hl₃⟩ := ih nextCurr hpos.lt
+    refine ⟨(s.slice pos nextCurr hpos.le).copy :: l, ?_, hl₂, ?_⟩
+    · simpa only [List.mem_cons, forall_eq_or_imp] using ⟨hpos.matches_slice, hl₁⟩
+    · simpa [String.append_assoc, ← hl₃] using (Slice.Pos.sliceFrom _ _ hpos.le).splits.eq_append
+  | none =>
+    rw [skipWhile_eq]
+    simpa [hpos] using ⟨[], by simp, by simpa using hpos, by simp⟩
+
+theorem skipPrefixWhile_eq_skipWhile_startPos {ρ : Type} {pat : ρ} [ForwardPattern pat] {s : Slice} :
+    s.skipPrefixWhile pat = s.startPos.skipWhile pat :=
+  (rfl)
+
+@[simp]
+theorem cast_skipPrefixWhile {ρ : Type} {pat : ρ} [PatternModel pat] [ForwardPattern pat]
+    [LawfulForwardPatternModel pat] {s t : Slice} (hst : s.copy = t.copy) :
+    (s.skipPrefixWhile pat).cast hst = t.skipPrefixWhile pat := by
+  simp [skipPrefixWhile_eq_skipWhile_startPos, ← Pos.skipWhile_cast]
+
+theorem Pattern.Model.exists_eq_of_skipPrefixWhile_eq {ρ : Type} {pat : ρ} [PatternModel pat] [StrictPatternModel pat] [ForwardPattern pat]
+    [LawfulForwardPatternModel pat] {s : Slice} {res : s.Pos} (h : s.skipPrefixWhile pat = res) :
+    ∃ (l : List String),
+      (∀ t ∈ l, PatternModel.Matches pat t) ∧ ¬MatchesAt pat res ∧ s.copy = String.join l ++ (s.sliceFrom res).copy := by
+  rw [skipPrefixWhile_eq_skipWhile_startPos] at h
+  simpa using Pos.exists_eq_of_skipWhile_eq h
+
+theorem dropWhile_eq_sliceFrom_skipPrefixWhile {ρ : Type} {pat : ρ} [ForwardPattern pat] {s : Slice} :
+    s.dropWhile pat = s.sliceFrom (s.skipPrefixWhile pat) :=
+  (rfl)
+
+theorem dropWhile_congr {ρ : Type} {pat : ρ} [PatternModel pat] [ForwardPattern pat] [LawfulForwardPatternModel pat]
+    {s t : Slice} (hst : s.copy = t.copy) : (s.dropWhile pat).copy = (t.dropWhile pat).copy := by
+  rw [dropWhile_eq_sliceFrom_skipPrefixWhile, dropWhile_eq_sliceFrom_skipPrefixWhile,
+    ← cast_skipPrefixWhile hst, copy_sliceFrom_cast]
+
+theorem Pattern.Model.exists_of_dropWhile_eq {ρ : Type} {pat : ρ} [PatternModel pat] [StrictPatternModel pat] [ForwardPattern pat]
+    [LawfulForwardPatternModel pat] {s res : Slice} (h : s.dropWhile pat = res) :
+    ∃ (l : List String), (∀ t ∈ l, PatternModel.Matches pat t) ∧ res.startsWith pat = false ∧ s.copy = String.join l ++ res.copy := by
+  subst res
+  simpa [dropWhile_eq_sliceFrom_skipPrefixWhile, Pattern.Model.startsWith_eq_false_iff,
+    matchesAt_iff_matchesAt_ofSliceFrom] using exists_eq_of_skipPrefixWhile_eq (rfl : s.skipPrefixWhile pat = _)
+
+theorem takeWhile_eq_sliceTo_skipPrefixWhile {ρ : Type} {pat : ρ} [ForwardPattern pat] {s : Slice} :
+    s.takeWhile pat = s.sliceTo (s.skipPrefixWhile pat) :=
+  (rfl)
+
+theorem takeWhile_congr {ρ : Type} {pat : ρ} [PatternModel pat] [ForwardPattern pat] [LawfulForwardPatternModel pat]
+    {s t : Slice} (hst : s.copy = t.copy) : (s.takeWhile pat).copy = (t.takeWhile pat).copy := by
+  rw [takeWhile_eq_sliceTo_skipPrefixWhile, takeWhile_eq_sliceTo_skipPrefixWhile,
+    ← cast_skipPrefixWhile hst, copy_sliceTo_cast]
+
 theorem skipSuffix?_eq_backwardPatternSkipSuffix? {ρ : Type} {pat : ρ} [BackwardPattern pat] {s : Slice} :
     s.skipSuffix? pat = BackwardPattern.skipSuffix? pat s := (rfl)
 
@@ -129,11 +289,119 @@ end Slice
 theorem skipPrefix?_eq_skipPrefix?_toSlice {ρ : Type} {pat : ρ} [ForwardPattern pat] {s : String} :
     s.skipPrefix? pat = (s.toSlice.skipPrefix? pat).map Pos.ofToSlice := (rfl)
 
+theorem skipPrefix?_toSlice {ρ : Type} {pat : ρ} [ForwardPattern pat] {s : String} :
+    s.toSlice.skipPrefix? pat = (s.skipPrefix? pat).map Pos.toSlice := by
+  simp [skipPrefix?_eq_skipPrefix?_toSlice]
+
+theorem Slice.skipPrefix?_copy {ρ : Type} {pat : ρ} [ForwardPattern pat] [PatternModel pat] [LawfulForwardPatternModel pat]
+    {s : Slice} : s.copy.skipPrefix? pat = (s.skipPrefix? pat).map Slice.Pos.copy := by
+  rw [skipPrefix?_eq_skipPrefix?_toSlice, Slice.skipPrefix?_congr String.copy_toSlice, Option.map_map]
+  congr 1
+  ext
+  simp
+
 theorem startsWith_eq_startsWith_toSlice {ρ : Type} {pat : ρ} [ForwardPattern pat] {s : String} :
     s.startsWith pat = s.toSlice.startsWith pat := (rfl)
 
+@[simp]
+theorem startsWith_toSlice {ρ : Type} {pat : ρ} [ForwardPattern pat] {s : String} :
+    s.toSlice.startsWith pat = s.startsWith pat := (rfl)
+
+@[simp]
+theorem Slice.startsWith_copy {ρ : Type} {pat : ρ} [ForwardPattern pat] [PatternModel pat] [LawfulForwardPatternModel pat]
+    {s : Slice} : s.copy.startsWith pat = s.startsWith pat := by
+  simpa only [← startsWith_toSlice] using Slice.startsWith_congr (by simp)
+
 theorem dropPrefix?_eq_dropPrefix?_toSlice {ρ : Type} {pat : ρ} [ForwardPattern pat] {s : String} :
     s.dropPrefix? pat = s.toSlice.dropPrefix? pat := (rfl)
+
+@[simp]
+theorem dropPrefix?_toSlice {ρ : Type} {pat : ρ} [ForwardPattern pat] {s : String} :
+    s.toSlice.dropPrefix? pat = s.dropPrefix? pat := (rfl)
+
+@[simp]
+theorem Slice.copy_dropPrefix?_copy {ρ : Type} {pat : ρ} [ForwardPattern pat] [PatternModel pat]
+    [LawfulForwardPatternModel pat] {s : Slice} :
+    (s.copy.dropPrefix? pat).map String.Slice.copy = (s.dropPrefix? pat).map String.Slice.copy := by
+  rw [dropPrefix?_eq_dropPrefix?_toSlice, Slice.dropPrefix?_congr String.copy_toSlice]
+
+theorem skip?_eq_skip?_toSlice {ρ : Type} {pat : ρ} [ForwardPattern pat] {s : String} {pos : s.Pos} :
+    pos.skip? pat = (pos.toSlice.skip? pat).map Pos.ofToSlice := (rfl)
+
+theorem skip?_toSlice {ρ : Type} {pat : ρ} [ForwardPattern pat] {s : String} {pos : s.Pos} :
+    pos.toSlice.skip? pat = (pos.skip? pat).map Pos.toSlice := by
+  simp [skip?_eq_skip?_toSlice]
+
+-- TODO: move
+@[simp]
+theorem Slice.Pos.cast_toSlice_copy {s : Slice} {pos : s.Pos} :
+    pos.copy.toSlice.cast (by simp) = pos := by
+  ext; simp
+
+theorem Slice.Pos.skip?_copy {ρ : Type} {pat : ρ} [ForwardPattern pat] [PatternModel pat]
+    [LawfulForwardPatternModel pat] {s : Slice} {pos : s.Pos} :
+    pos.copy.skip? pat = (pos.skip? pat).map Slice.Pos.copy := by
+  rw [skip?_eq_skip?_toSlice, Slice.Pos.skip?_congr (hst := String.copy_toSlice), cast_toSlice_copy, Option.map_map]
+  congr 1
+  ext
+  simp
+
+theorem Pos.skipWhile_eq_skipWhile_toSlice {ρ : Type} {pat : ρ} [ForwardPattern pat] {s : String}
+    {pos : s.Pos} : pos.skipWhile pat = Pos.ofToSlice (pos.toSlice.skipWhile pat) := (rfl)
+
+theorem Pos.skipWhile_toSlice {ρ : Type} {pat : ρ} [ForwardPattern pat] {s : String}
+    {pos : s.Pos} : pos.toSlice.skipWhile pat = Pos.toSlice (pos.skipWhile pat) := by
+  simp [Pos.skipWhile_eq_skipWhile_toSlice]
+
+theorem Slice.Pos.skipWhile_copy {ρ : Type} {pat : ρ} [ForwardPattern pat] [PatternModel pat]
+    [LawfulForwardPatternModel pat] {s : Slice}
+    {pos : s.Pos} : pos.copy.skipWhile pat = (pos.skipWhile pat).copy := by
+  rw [Pos.skipWhile_eq_skipWhile_toSlice, Slice.Pos.skipWhile_congr String.copy_toSlice,
+    cast_toSlice_copy]
+  ext
+  simp
+
+theorem skipPrefixWhile_eq_skipPrefixWhile_toSlice {ρ : Type} {pat : ρ} [ForwardPattern pat] {s : String} :
+    s.skipPrefixWhile pat = Pos.ofToSlice (s.toSlice.skipPrefixWhile pat) := (rfl)
+
+theorem skipPrefixWhile_toSlice {ρ : Type} {pat : ρ} [ForwardPattern pat] {s : String} :
+    s.toSlice.skipPrefixWhile pat = Pos.toSlice (s.skipPrefixWhile pat) := by
+  simp [skipPrefixWhile_eq_skipPrefixWhile_toSlice]
+
+theorem Slice.skipPrefixWhile_copy {ρ : Type} {pat : ρ} [ForwardPattern pat] [PatternModel pat]
+    [LawfulForwardPatternModel pat] {s : Slice} :
+    s.copy.skipPrefixWhile pat = (s.skipPrefixWhile pat).copy := by
+  rw [skipPrefixWhile_eq_skipPrefixWhile_toSlice, ← cast_skipPrefixWhile String.copy_toSlice.symm]
+  ext
+  simp [-cast_skipPrefixWhile]
+
+theorem dropWhile_eq_dropWhile_toSlice {ρ : Type} {pat : ρ} [ForwardPattern pat] {s : String} :
+    s.dropWhile pat = s.toSlice.dropWhile pat := (rfl)
+
+@[simp]
+theorem dropWhile_toSlice {ρ : Type} {pat : ρ} [ForwardPattern pat] {s : String} :
+    s.toSlice.dropWhile pat = s.dropWhile pat := by
+  simp [dropWhile_eq_dropWhile_toSlice]
+
+@[simp]
+theorem Slice.dropWhile_copy {ρ : Type} {pat : ρ} [ForwardPattern pat] [PatternModel pat]
+    [LawfulForwardPatternModel pat] {s : Slice} :
+    (s.copy.dropWhile pat).copy = (s.dropWhile pat).copy := by
+  simpa [← dropWhile_toSlice] using Slice.dropWhile_congr (by simp)
+
+theorem takeWhile_eq_takeWhile_toSlice {ρ : Type} {pat : ρ} [ForwardPattern pat] {s : String} :
+    s.takeWhile pat = s.toSlice.takeWhile pat := (rfl)
+
+@[simp]
+theorem takeWhile_toSlice {ρ : Type} {pat : ρ} [ForwardPattern pat] {s : String} :
+    s.toSlice.takeWhile pat = s.takeWhile pat := by
+  simp [takeWhile_eq_takeWhile_toSlice]
+
+@[simp]
+theorem Slice.takeWhile_copy {ρ : Type} {pat : ρ} [ForwardPattern pat] [PatternModel pat]
+    [LawfulForwardPatternModel pat] {s : Slice} :
+    (s.copy.takeWhile pat).copy = (s.takeWhile pat).copy := by
+  simpa [← takeWhile_toSlice] using Slice.takeWhile_congr (by simp)
 
 theorem skipSuffix?_eq_skipSuffix?_toSlice {ρ : Type} {pat : ρ} [BackwardPattern pat] {s : String} :
     s.skipSuffix? pat = (s.toSlice.skipSuffix? pat).map Pos.ofToSlice := (rfl)
@@ -143,5 +411,19 @@ theorem endsWith_eq_endsWith_toSlice {ρ : Type} {pat : ρ} [BackwardPattern pat
 
 theorem dropSuffix?_eq_dropSuffix?_toSlice {ρ : Type} {pat : ρ} [BackwardPattern pat] {s : String} :
     s.dropSuffix? pat = s.toSlice.dropSuffix? pat := (rfl)
+
+namespace Slice
+
+theorem Pattern.Model.exists_of_takeWhile_eq {ρ : Type} {pat : ρ} [PatternModel pat] [StrictPatternModel pat] [ForwardPattern pat]
+    [LawfulForwardPatternModel pat] {s res : Slice} (h : s.takeWhile pat = res) :
+    ∃ (l : List String) (r : String), (∀ t ∈ l, PatternModel.Matches pat t) ∧ r.startsWith pat = false ∧ res.copy = String.join l ∧ s.copy = res.copy ++ r := by
+  subst res
+  obtain ⟨t, ht₁, ht₂, ht₃⟩ := exists_eq_of_skipPrefixWhile_eq (rfl : s.skipPrefixWhile pat = _)
+  simp only [takeWhile_eq_sliceTo_skipPrefixWhile, exists_and_left]
+  refine ⟨t, ht₁, (s.sliceFrom (s.skipPrefixWhile pat)).copy, ?_, ?_, (s.skipPrefixWhile pat).splits.eq_append⟩
+  · simpa [startsWith_eq_false_iff, matchesAt_iff_matchesAt_ofSliceFrom]
+  · simpa [(s.skipPrefixWhile pat).splits.eq_append] using ht₃
+
+end Slice
 
 end String
